HW4 (WIP) and moved superduniform to a separate file

lecture-files-fixed/Lecture_04/Lecture.ec
@@ -1,18 +1,19 @@
 require import AllCore.
-(* require import Fun. *)
-(* import Fun.Bijections. *)
 require FSet.
-(* require ISet. *)
 require Distr.
-
-(* print FSet.Duni.duni . *)
 
 type D.
 clone Distr.MFinite as DD with
   type t <= D.
-(* Implicitly axiomatized finiteness: *)
-print DD.Support.enum_spec.
-(* If we wanted not to axiomatize it, we would add "proof *" before the . in the clone command *)
+
+(* Implicitly axiomatized finiteness:
+If we wanted not to axiomatize it,
+we would add "proof *" before the . in the clone command
+Like so:
+
+clone Distr.MFinite as DD with
+  type t <= D
+  proof *. *)
 
 op f : D -> D.
 axiom f_bij: bijective f.
@@ -33,12 +34,14 @@ module Game = {
 lemma adv_silly:
     hoare [ Game.owp : true ==> res<>true ].
 proof.
-(*  proc.
+(*
+  proc.
   wp 2.
   wp 1.
   rnd.
   skip.
-  smt. *)
+  smt.
+*)
   proc; auto; smt.
 qed.
 
@@ -60,63 +63,4 @@ lemma adv_silly2:
     hoare [ Game2.owp : true ==> res<>true ].
 proof.
   proc; auto; smt.
-qed.
-
-import List.
-import Distr.
-print duniform.
-lemma test (x:'a): mu1 (duniform []) x = 0%r.
-    smt.
-qed.
-
-lemma test2 (x:'a) l:
-    (x \in l)%List =>
-    mu1 (duniform l) x > 0%r.
-    smt.
-qed.
-
-type 'a set = 'a -> bool.
-
-op superduniform (s : 'a set) : 'a distr =
-  duniform (choiceb (fun l => s = List.mem l) []).
-
-
-op finite (s: 'a set) : bool =
-  exists l, s = List.mem l.
-
-(* lemma finlist (s:'a set): *)
-(*     finite s => exists l, s = List.mem l. *)
-(*   smt. *)
-(* qed. *)
-
-lemma link (l:'a list):
-    duniform l = superduniform (List.mem l).
-    rewrite /superduniform.
-    pose l0 := choiceb (fun (l0 : 'a list) => mem l = mem l0) [].
-    rewrite -eq_duniformP.
-    have Hl0: mem l = mem l0.
-    smt.
-    rewrite Hl0.
-    trivial.
-qed.
-    
-lemma test3 (x:'a) s:
-    finite s =>
-    s x =>
-    mu1 (superduniform s) x > 0%r.
-    
-    move => Hfin Hmem.
-    have Hex: exists l, s = List.mem l.
-    rewrite /finite in Hfin.
-    apply Hfin.
-    elim Hex.
-
-    move => l Hl.
-    rewrite Hl.
-    rewrite -link.
-
-    apply test2.
-    rewrite -Hl.
-    apply Hmem.
-
 qed.
