lecture-files-fixed/Lecture_04/superduniform.ec
@@ -1,0 +1,63 @@
+require import AllCore.
+require import Distr.
+import List.
+
+print duniform.
+
+  (* This file consists of the ideas and exploration when working with lists and distributions *)
+
+lemma test (x:'a): mu1 (duniform []) x = 0%r.
+    smt.
+qed.
+
+lemma test2 (x:'a) l:
+    (x \in l)%List =>
+    mu1 (duniform l) x > 0%r.
+    smt.
+qed.
+
+type 'a set = 'a -> bool.
+
+op superduniform (s : 'a set) : 'a distr =
+  duniform (choiceb (fun l => s = List.mem l) []).
+
+
+op finite (s: 'a set) : bool =
+  exists l, s = List.mem l.
+
+(* lemma finlist (s:'a set): *)
+(*     finite s => exists l, s = List.mem l. *)
+(*   smt. *)
+(* qed. *)
+
+lemma link (l:'a list):
+    duniform l = superduniform (List.mem l).
+    rewrite /superduniform.
+    pose l0 := choiceb (fun (l0 : 'a list) => mem l = mem l0) [].
+    rewrite -eq_duniformP.
+    have Hl0: mem l = mem l0.
+    smt.
+    rewrite Hl0.
+    trivial.
+qed.
+    
+lemma test3 (x:'a) s:
+    finite s =>
+    s x =>
+    mu1 (superduniform s) x > 0%r.
+    
+    move => Hfin Hmem.
+    have Hex: exists l, s = List.mem l.
+    rewrite /finite in Hfin.
+    apply Hfin.
+    elim Hex.
+
+    move => l Hl.
+    rewrite Hl.
+    rewrite -link.
+
+    apply test2.
+    rewrite -Hl.
+    apply Hmem.
+
+qed.
